src/HOL/Induct/Comb.thy
@@ -1,74 +1,220 @@
-(*  Title:      HOL/ex/Comb.thy
+(*  Title:      HOL/Induct/Comb.thy
     ID:         $Id$
     Author:     Lawrence C Paulson
     Copyright   1996  University of Cambridge
-
-Combinatory Logic example: the Church-Rosser Theorem
-Curiously, combinators do not include free variables.
-
-Example taken from
-    J. Camilleri and T. F. Melham.
-    Reasoning with Inductively Defined Relations in the HOL Theorem Prover.
-    Report 265, University of Cambridge Computer Laboratory, 1992.
 *)
 
+header {* Combinatory Logic example: the Church-Rosser Theorem *}
 
-Comb = Main +
+theory Comb = Main:
 
-(** Datatype definition of combinators S and K, with infixed application **)
+text {*
+  Curiously, combinators do not include free variables.
+
+  Example taken from \cite{camilleri-melham}.
+
+HOL system proofs may be found in the HOL distribution at
+   .../contrib/rule-induction/cl.ml
+*}
+
+subsection {* Definitions *}
+
+text {* Datatype definition of combinators @{text S} and @{text K}. *}
+
 datatype comb = K
               | S
               | "##" comb comb (infixl 90)
 
-(** Inductive definition of contractions, -1->
-             and (multi-step) reductions, --->
-**)
+text {*
+  Inductive definition of contractions, @{text "-1->"} and
+  (multi-step) reductions, @{text "--->"}.
+*}
+
 consts
   contract  :: "(comb*comb) set"
-  "-1->"    :: [comb,comb] => bool   (infixl 50)
-  "--->"    :: [comb,comb] => bool   (infixl 50)
+  "-1->"    :: "[comb,comb] => bool"   (infixl 50)
+  "--->"    :: "[comb,comb] => bool"   (infixl 50)
 
 translations
-  "x -1-> y" == "(x,y) : contract"
-  "x ---> y" == "(x,y) : contract^*"
+  "x -1-> y" == "(x,y) \<in> contract"
+  "x ---> y" == "(x,y) \<in> contract^*"
 
 inductive contract
-  intrs
-    K     "K##x##y -1-> x"
-    S     "S##x##y##z -1-> (x##z)##(y##z)"
-    Ap1   "x-1->y ==> x##z -1-> y##z"
-    Ap2   "x-1->y ==> z##x -1-> z##y"
+  intros
+    K:     "K##x##y -1-> x"
+    S:     "S##x##y##z -1-> (x##z)##(y##z)"
+    Ap1:   "x-1->y ==> x##z -1-> y##z"
+    Ap2:   "x-1->y ==> z##x -1-> z##y"
 
+text {*
+  Inductive definition of parallel contractions, @{text "=1=>"} and
+  (multi-step) parallel reductions, @{text "===>"}.
+*}
 
-(** Inductive definition of parallel contractions, =1=>
-             and (multi-step) parallel reductions, ===>
-**)
 consts
   parcontract :: "(comb*comb) set"
-  "=1=>"    :: [comb,comb] => bool   (infixl 50)
-  "===>"    :: [comb,comb] => bool   (infixl 50)
+  "=1=>"      :: "[comb,comb] => bool"   (infixl 50)
+  "===>"      :: "[comb,comb] => bool"   (infixl 50)
 
 translations
-  "x =1=> y" == "(x,y) : parcontract"
-  "x ===> y" == "(x,y) : parcontract^*"
+  "x =1=> y" == "(x,y) \<in> parcontract"
+  "x ===> y" == "(x,y) \<in> parcontract^*"
 
 inductive parcontract
-  intrs
-    refl  "x =1=> x"
-    K     "K##x##y =1=> x"
-    S     "S##x##y##z =1=> (x##z)##(y##z)"
-    Ap    "[| x=1=>y;  z=1=>w |] ==> x##z =1=> y##w"
+  intros
+    refl:  "x =1=> x"
+    K:     "K##x##y =1=> x"
+    S:     "S##x##y##z =1=> (x##z)##(y##z)"
+    Ap:    "[| x=1=>y;  z=1=>w |] ==> x##z =1=> y##w"
 
+text {*
+  Misc definitions.
+*}
 
-(*Misc definitions*)
 constdefs
   I :: comb
   "I == S##K##K"
 
-  (*confluence; Lambda/Commutation treats this more abstractly*)
   diamond   :: "('a * 'a)set => bool"	
-  "diamond(r) == ALL x y. (x,y):r --> 
-                  (ALL y'. (x,y'):r --> 
-                    (EX z. (y,z):r & (y',z) : r))"
+    --{*confluence; Lambda/Commutation treats this more abstractly*}
+  "diamond(r) == \<forall>x y. (x,y) \<in> r --> 
+                  (\<forall>y'. (x,y') \<in> r --> 
+                    (\<exists>z. (y,z) \<in> r & (y',z) \<in> r))"
+
+
+subsection {*Reflexive/Transitive closure preserves Church-Rosser property*}
+
+text{*So does the Transitive closure, with a similar proof*}
+
+text{*Strip lemma.  
+   The induction hypothesis covers all but the last diamond of the strip.*}
+lemma diamond_strip_lemmaE [rule_format]: 
+    "[| diamond(r);  (x,y) \<in> r^* |] ==>   
+          \<forall>y'. (x,y') \<in> r --> (\<exists>z. (y',z) \<in> r^* & (y,z) \<in> r)"
+apply (unfold diamond_def)
+apply (erule rtrancl_induct, blast, clarify)
+apply (drule spec, drule mp, assumption)
+apply (blast intro: rtrancl_trans [OF _ r_into_rtrancl])
+done
+
+lemma diamond_rtrancl: "diamond(r) ==> diamond(r^*)"
+apply (simp (no_asm_simp) add: diamond_def)
+apply (rule impI [THEN allI, THEN allI])
+apply (erule rtrancl_induct, blast)
+apply (best intro: rtrancl_trans [OF _ r_into_rtrancl] 
+            elim: diamond_strip_lemmaE [THEN exE])
+done
+
+
+subsection {* Non-contraction results *}
+
+text {* Derive a case for each combinator constructor. *}
+
+inductive_cases
+      K_contractE [elim!]: "K -1-> r"
+  and S_contractE [elim!]: "S -1-> r"
+  and Ap_contractE [elim!]: "p##q -1-> r"
+
+declare contract.K [intro!] contract.S [intro!]
+declare contract.Ap1 [intro] contract.Ap2 [intro]
+
+lemma I_contract_E [elim!]: "I -1-> z ==> P"
+by (unfold I_def, blast)
+
+lemma K1_contractD [elim!]: "K##x -1-> z ==> (\<exists>x'. z = K##x' & x -1-> x')"
+by blast
+
+lemma Ap_reduce1 [intro]: "x ---> y ==> x##z ---> y##z"
+apply (erule rtrancl_induct)
+apply (blast intro: rtrancl_trans)+
+done
+
+lemma Ap_reduce2 [intro]: "x ---> y ==> z##x ---> z##y"
+apply (erule rtrancl_induct)
+apply (blast intro: rtrancl_trans)+
+done
+
+(** Counterexample to the diamond property for -1-> **)
+
+lemma KIII_contract1: "K##I##(I##I) -1-> I"
+by (rule contract.K)
+
+lemma KIII_contract2: "K##I##(I##I) -1-> K##I##((K##I)##(K##I))"
+by (unfold I_def, blast)
+
+lemma KIII_contract3: "K##I##((K##I)##(K##I)) -1-> I"
+by blast
+
+lemma not_diamond_contract: "~ diamond(contract)"
+apply (unfold diamond_def) 
+apply (best intro: KIII_contract1 KIII_contract2 KIII_contract3)
+done
+
+
+subsection {* Results about Parallel Contraction *}
+
+text {* Derive a case for each combinator constructor. *}
+
+inductive_cases
+      K_parcontractE [elim!]: "K =1=> r"
+  and S_parcontractE [elim!]: "S =1=> r"
+  and Ap_parcontractE [elim!]: "p##q =1=> r"
+
+declare parcontract.intros [intro]
+
+(*** Basic properties of parallel contraction ***)
+
+subsection {* Basic properties of parallel contraction *}
+
+lemma K1_parcontractD [dest!]: "K##x =1=> z ==> (\<exists>x'. z = K##x' & x =1=> x')"
+by blast
+
+lemma S1_parcontractD [dest!]: "S##x =1=> z ==> (\<exists>x'. z = S##x' & x =1=> x')"
+by blast
+
+lemma S2_parcontractD [dest!]:
+     "S##x##y =1=> z ==> (\<exists>x' y'. z = S##x'##y' & x =1=> x' & y =1=> y')"
+by blast
+
+text{*The rules above are not essential but make proofs much faster*}
+
+text{*Church-Rosser property for parallel contraction*}
+lemma diamond_parcontract: "diamond parcontract"
+apply (unfold diamond_def)
+apply (rule impI [THEN allI, THEN allI])
+apply (erule parcontract.induct, fast+)
+done
+
+text {*
+  \medskip Equivalence of @{prop "p ---> q"} and @{prop "p ===> q"}.
+*}
+
+lemma contract_subset_parcontract: "contract <= parcontract"
+apply (rule subsetI)
+apply (simp only: split_tupled_all)
+apply (erule contract.induct, blast+)
+done
+
+text{*Reductions: simply throw together reflexivity, transitivity and
+  the one-step reductions*}
+
+declare r_into_rtrancl [intro]  rtrancl_trans [intro]
+
+(*Example only: not used*)
+lemma reduce_I: "I##x ---> x"
+by (unfold I_def, blast)
+
+lemma parcontract_subset_reduce: "parcontract <= contract^*"
+apply (rule subsetI)
+apply (simp only: split_tupled_all)
+apply (erule parcontract.induct , blast+)
+done
+
+lemma reduce_eq_parreduce: "contract^* = parcontract^*"
+by (rule equalityI contract_subset_parcontract [THEN rtrancl_mono] 
+         parcontract_subset_reduce [THEN rtrancl_subset_rtrancl])+
+
+lemma diamond_reduce: "diamond(contract^*)"
+by (simp add: reduce_eq_parreduce diamond_rtrancl diamond_parcontract)
 
 end
