src/HOL/Induct/LFilter.thy
@@ -2,28 +2,271 @@
     ID:         $Id$
     Author:     Lawrence C Paulson, Cambridge University Computer Laboratory
     Copyright   1997  University of Cambridge
-
-The "filter" functional for coinductive lists
-  --defined by a combination of induction and coinduction
 *)
 
-LFilter = LList +
+header {*The "filter" functional for coinductive lists
+  --defined by a combination of induction and coinduction*}
+
+theory LFilter = LList:
 
 consts
   findRel	:: "('a => bool) => ('a llist * 'a llist)set"
 
 inductive "findRel p"
-  intrs
-    found  "p x ==> (LCons x l, LCons x l) : findRel p"
-    seek   "[| ~p x;  (l,l') : findRel p |] ==> (LCons x l, l') : findRel p"
+  intros
+    found:  "p x ==> (LCons x l, LCons x l) \<in> findRel p"
+    seek:   "[| ~p x;  (l,l') \<in> findRel p |] ==> (LCons x l, l') \<in> findRel p"
+
+declare findRel.intros [intro]
 
 constdefs
-  find		:: ['a => bool, 'a llist] => 'a llist
+  find    :: "['a => bool, 'a llist] => 'a llist"
     "find p l == @l'. (l,l'): findRel p | (l' = LNil & l ~: Domain(findRel p))"
 
-  lfilter	:: ['a => bool, 'a llist] => 'a llist
+  lfilter :: "['a => bool, 'a llist] => 'a llist"
     "lfilter p l == llist_corec l (%l. case find p l of
                                             LNil => None
                                           | LCons y z => Some(y,z))"
+
+
+subsection {* findRel: basic laws *}
+
+inductive_cases
+  findRel_LConsE [elim!]: "(LCons x l, l'') \<in> findRel p"
+
+
+lemma findRel_functional [rule_format]:
+     "(l,l'): findRel p ==> (l,l''): findRel p --> l'' = l'"
+by (erule findRel.induct, auto)
+
+lemma findRel_imp_LCons [rule_format]:
+     "(l,l'): findRel p ==> \<exists>x l''. l' = LCons x l'' & p x"
+by (erule findRel.induct, auto)
+
+lemma findRel_LNil [elim!]: "(LNil,l): findRel p ==> R"
+by (blast elim: findRel.cases)
+
+
+subsection {* Properties of Domain (findRel p) *}
+
+lemma LCons_Domain_findRel [simp]:
+     "LCons x l \<in> Domain(findRel p) = (p x | l \<in> Domain(findRel p))"
+by auto
+
+lemma Domain_findRel_iff:
+     "(l \<in> Domain (findRel p)) = (\<exists>x l'. (l, LCons x l') \<in> findRel p &  p x)" 
+by (blast dest: findRel_imp_LCons) 
+
+lemma Domain_findRel_mono:
+    "[| !!x. p x ==> q x |] ==> Domain (findRel p) <= Domain (findRel q)"
+apply clarify
+apply (erule findRel.induct, blast+)
+done
+
+
+subsection {* find: basic equations *}
+
+lemma find_LNil [simp]: "find p LNil = LNil"
+by (unfold find_def, blast)
+
+lemma findRel_imp_find [simp]: "(l,l') \<in> findRel p ==> find p l = l'"
+apply (unfold find_def)
+apply (blast dest: findRel_functional)
+done
+
+lemma find_LCons_found: "p x ==> find p (LCons x l) = LCons x l"
+by (blast intro: findRel_imp_find)
+
+lemma diverge_find_LNil [simp]: "l ~: Domain(findRel p) ==> find p l = LNil"
+by (unfold find_def, blast)
+
+lemma find_LCons_seek: "~ (p x) ==> find p (LCons x l) = find p l"
+apply (case_tac "LCons x l \<in> Domain (findRel p) ")
+ apply auto 
+apply (blast intro: findRel_imp_find)
+done
+
+lemma find_LCons [simp]:
+     "find p (LCons x l) = (if p x then LCons x l else find p l)"
+by (simp add: find_LCons_seek find_LCons_found)
+
+
+
+subsection {* lfilter: basic equations *}
+
+lemma lfilter_LNil [simp]: "lfilter p LNil = LNil"
+by (rule lfilter_def [THEN def_llist_corec, THEN trans], simp)
+
+lemma diverge_lfilter_LNil [simp]:
+     "l ~: Domain(findRel p) ==> lfilter p l = LNil"
+by (rule lfilter_def [THEN def_llist_corec, THEN trans], simp)
+
+lemma lfilter_LCons_found:
+     "p x ==> lfilter p (LCons x l) = LCons x (lfilter p l)"
+by (rule lfilter_def [THEN def_llist_corec, THEN trans], simp)
+
+lemma findRel_imp_lfilter [simp]:
+     "(l, LCons x l') \<in> findRel p ==> lfilter p l = LCons x (lfilter p l')"
+by (rule lfilter_def [THEN def_llist_corec, THEN trans], simp)
+
+lemma lfilter_LCons_seek: "~ (p x) ==> lfilter p (LCons x l) = lfilter p l"
+apply (rule lfilter_def [THEN def_llist_corec, THEN trans], simp)
+apply (case_tac "LCons x l \<in> Domain (findRel p) ")
+ apply (simp add: Domain_findRel_iff, auto) 
+done
+
+lemma lfilter_LCons [simp]:
+     "lfilter p (LCons x l) =  
+          (if p x then LCons x (lfilter p l) else lfilter p l)"
+by (simp add: lfilter_LCons_found lfilter_LCons_seek)
+
+declare llistD_Fun_LNil_I [intro!] llistD_Fun_LCons_I [intro!]
+
+
+lemma lfilter_eq_LNil: "lfilter p l = LNil ==> l ~: Domain(findRel p)" 
+apply (auto iff: Domain_findRel_iff)
+apply (rotate_tac 1, simp) 
+done
+
+lemma lfilter_eq_LCons [rule_format]:
+     "lfilter p l = LCons x l' -->      
+               (\<exists>l''. l' = lfilter p l'' & (l, LCons x l'') \<in> findRel p)"
+apply (subst lfilter_def [THEN def_llist_corec])
+apply (case_tac "l \<in> Domain (findRel p) ")
+ apply (auto iff: Domain_findRel_iff)
+done
+
+
+lemma lfilter_cases: "lfilter p l = LNil  |   
+          (\<exists>y l'. lfilter p l = LCons y (lfilter p l') & p y)"
+apply (case_tac "l \<in> Domain (findRel p) ")
+apply (auto iff: Domain_findRel_iff)
+done
+
+
+subsection {* lfilter: simple facts by coinduction *}
+
+lemma lfilter_K_True: "lfilter (%x. True) l = l"
+by (rule_tac l = "l" in llist_fun_equalityI, simp_all)
+
+lemma lfilter_idem: "lfilter p (lfilter p l) = lfilter p l"
+apply (rule_tac l = "l" in llist_fun_equalityI, simp_all)
+apply safe
+txt{*Cases: p x is true or false*}
+apply (rule lfilter_cases [THEN disjE])
+ apply (erule ssubst, auto)
+done
+
+
+subsection {* Numerous lemmas required to prove @{text lfilter_conj} *}
+
+lemma findRel_conj_lemma [rule_format]:
+     "(l,l') \<in> findRel q  
+      ==> l' = LCons x l'' --> p x --> (l,l') \<in> findRel (%x. p x & q x)"
+by (erule findRel.induct, auto)
+
+lemmas findRel_conj = findRel_conj_lemma [OF _ refl]
+
+lemma findRel_not_conj_Domain [rule_format]:
+     "(l,l'') \<in> findRel (%x. p x & q x)  
+      ==> (l, LCons x l') \<in> findRel q --> ~ p x --> 
+          l' \<in> Domain (findRel (%x. p x & q x))"
+by (erule findRel.induct, auto)
+
+lemma findRel_conj2 [rule_format]:
+     "(l,lxx) \<in> findRel q 
+      ==> lxx = LCons x lx --> (lx,lz) \<in> findRel(%x. p x & q x) --> ~ p x  
+          --> (l,lz) \<in> findRel (%x. p x & q x)"
+by (erule findRel.induct, auto)
+
+lemma findRel_lfilter_Domain_conj [rule_format]:
+     "(lx,ly) \<in> findRel p  
+      ==> \<forall>l. lx = lfilter q l --> l \<in> Domain (findRel(%x. p x & q x))"
+apply (erule findRel.induct)
+ apply (blast dest!: sym [THEN lfilter_eq_LCons] intro: findRel_conj, auto)
+apply (drule sym [THEN lfilter_eq_LCons], auto)
+apply (drule spec)
+apply (drule refl [THEN rev_mp])
+apply (blast intro: findRel_conj2)
+done
+
+
+lemma findRel_conj_lfilter [rule_format]:
+     "(l,l'') \<in> findRel(%x. p x & q x)  
+      ==> l'' = LCons y l' --> 
+          (lfilter q l, LCons y (lfilter q l')) \<in> findRel p"
+by (erule findRel.induct, auto)
+
+lemma lfilter_conj_lemma:
+     "(lfilter p (lfilter q l), lfilter (%x. p x & q x) l)   
+      \<in> llistD_Fun (range (%u. (lfilter p (lfilter q u),           
+                                lfilter (%x. p x & q x) u)))"
+apply (case_tac "l \<in> Domain (findRel q)")
+ apply (subgoal_tac [2] "l ~: Domain (findRel (%x. p x & q x))")
+  prefer 3 apply (blast intro: rev_subsetD [OF _ Domain_findRel_mono])
+ txt{*There are no qs in l: both lists are LNil*}
+ apply (simp_all add: Domain_findRel_iff, clarify) 
+txt{*case q x*}
+apply (case_tac "p x")
+ apply (simp_all add: findRel_conj [THEN findRel_imp_lfilter])
+ txt{*case q x and ~(p x) *}
+apply (case_tac "l' \<in> Domain (findRel (%x. p x & q x))")
+ txt{*subcase: there is no p&q in l' and therefore none in l*}
+ apply (subgoal_tac [2] "l ~: Domain (findRel (%x. p x & q x))")
+  prefer 3 apply (blast intro: findRel_not_conj_Domain)
+ apply (subgoal_tac [2] "lfilter q l' ~: Domain (findRel p) ")
+  prefer 3 apply (blast intro: findRel_lfilter_Domain_conj)
+ txt{*    ...and therefore too, no p in lfilter q l'.  Both results are Lnil*}
+ apply (simp_all add: Domain_findRel_iff, clarify) 
+txt{*subcase: there is a p&q in l' and therefore also one in l*}
+apply (subgoal_tac " (l, LCons xa l'a) \<in> findRel (%x. p x & q x) ")
+ prefer 2 apply (blast intro: findRel_conj2)
+apply (subgoal_tac " (lfilter q l', LCons xa (lfilter q l'a)) \<in> findRel p")
+ apply simp 
+apply (blast intro: findRel_conj_lfilter)
+done
+
+
+lemma lfilter_conj: "lfilter p (lfilter q l) = lfilter (%x. p x & q x) l"
+apply (rule_tac l = "l" in llist_fun_equalityI, simp_all)
+apply (blast intro: lfilter_conj_lemma rev_subsetD [OF _ llistD_Fun_mono])
+done
+
+
+subsection {* Numerous lemmas required to prove ??:
+     lfilter p (lmap f l) = lmap f (lfilter (%x. p(f x)) l)
+ *}
+
+lemma findRel_lmap_Domain:
+     "(l,l') \<in> findRel(%x. p (f x)) ==> lmap f l \<in> Domain(findRel p)"
+by (erule findRel.induct, auto)
+
+lemma lmap_eq_LCons [rule_format]: "lmap f l = LCons x l' -->      
+               (\<exists>y l''. x = f y & l' = lmap f l'' & l = LCons y l'')"
+apply (subst lmap_def [THEN def_llist_corec])
+apply (rule_tac l = "l" in llistE, auto)
+done
+
+
+lemma lmap_LCons_findRel_lemma [rule_format]:
+     "(lx,ly) \<in> findRel p
+      ==> \<forall>l. lmap f l = lx --> ly = LCons x l' -->  
+          (\<exists>y l''. x = f y & l' = lmap f l'' &        
+          (l, LCons y l'') \<in> findRel(%x. p(f x)))"
+apply (erule findRel.induct, simp_all)
+apply (blast dest!: lmap_eq_LCons)+
+done
+
+lemmas lmap_LCons_findRel = lmap_LCons_findRel_lemma [OF _ refl refl]
+
+lemma lfilter_lmap: "lfilter p (lmap f l) = lmap f (lfilter (p o f) l)"
+apply (rule_tac l = "l" in llist_fun_equalityI, simp_all)
+apply safe
+apply (case_tac "lmap f l \<in> Domain (findRel p)")
+ apply (simp add: Domain_findRel_iff, clarify)
+ apply (frule lmap_LCons_findRel, force) 
+apply (subgoal_tac "l ~: Domain (findRel (%x. p (f x)))", simp)
+apply (blast intro: findRel_lmap_Domain)
+done
 
 end
