src/HOL/Induct/PropLog.thy
@@ -1,45 +1,276 @@
-(*  Title:      HOL/ex/PropLog.thy
+(*  Title:      HOL/Induct/PropLog.thy
     ID:         $Id$
     Author:     Tobias Nipkow
-    Copyright   1994  TU Muenchen
-
-Inductive definition of propositional logic.
+    Copyright   1994  TU Muenchen & University of Cambridge
 *)
 
-PropLog = Main +
+header {* Meta-theory of propositional logic *}
+
+theory PropLog = Main:
+
+text {*
+  Datatype definition of propositional logic formulae and inductive
+  definition of the propositional tautologies.
+
+  Inductive definition of propositional logic.  Soundness and
+  completeness w.r.t.\ truth-tables.
+
+  Prove: If @{text "H |= p"} then @{text "G |= p"} where @{text "G \<in>
+  Fin(H)"}
+*}
+
+subsection {* The datatype of propositions *}
 
 datatype
-    'a pl = false | var 'a ("#_" [1000]) | "->" ('a pl) ('a pl) (infixr 90)
+    'a pl = false | var 'a ("#_" [1000]) | "->" "'a pl" "'a pl" (infixr 90)
+
+subsection {* The proof system *}
+
 consts
-  thms :: 'a pl set => 'a pl set
-  "|-"  :: ['a pl set, 'a pl] => bool   (infixl 50)
-  "|="  :: ['a pl set, 'a pl] => bool   (infixl 50)
-  eval  :: ['a set, 'a pl] => bool      ("_[[_]]" [100,0] 100)
-  hyps  :: ['a pl, 'a set] => 'a pl set
+  thms  :: "'a pl set => 'a pl set"
+  "|-"  :: "['a pl set, 'a pl] => bool"   (infixl 50)
 
 translations
-  "H |- p" == "p : thms(H)"
+  "H |- p" == "p \<in> thms(H)"
 
 inductive "thms(H)"
-  intrs
-  H   "p:H ==> H |- p"
-  K   "H |- p->q->p"
-  S   "H |- (p->q->r) -> (p->q) -> p->r"
-  DN  "H |- ((p->false) -> false) -> p"
-  MP  "[| H |- p->q; H |- p |] ==> H |- q"
+  intros
+  H [intro]:  "p\<in>H ==> H |- p"
+  K:          "H |- p->q->p"
+  S:          "H |- (p->q->r) -> (p->q) -> p->r"
+  DN:         "H |- ((p->false) -> false) -> p"
+  MP:         "[| H |- p->q; H |- p |] ==> H |- q"
 
-defs
-  sat_def  "H |= p  ==  (!tt. (!q:H. tt[[q]]) --> tt[[p]])"
+subsection {* The semantics *}
 
-primrec
-         "tt[[false]] = False"
-         "tt[[#v]]    = (v:tt)"
-eval_imp "tt[[p->q]]  = (tt[[p]] --> tt[[q]])"
+subsubsection {* Semantics of propositional logic. *}
+
+consts
+  eval  :: "['a set, 'a pl] => bool"      ("_[[_]]" [100,0] 100)
+
+primrec     "tt[[false]] = False"
+	    "tt[[#v]]    = (v \<in> tt)"
+  eval_imp: "tt[[p->q]]  = (tt[[p]] --> tt[[q]])"
+
+text {*
+  A finite set of hypotheses from @{text t} and the @{text Var}s in
+  @{text p}.
+*}
+
+consts
+  hyps  :: "['a pl, 'a set] => 'a pl set"
 
 primrec
   "hyps false  tt = {}"
-  "hyps (#v)   tt = {if v:tt then #v else #v->false}"
+  "hyps (#v)   tt = {if v \<in> tt then #v else #v->false}"
   "hyps (p->q) tt = hyps p tt Un hyps q tt"
+
+subsubsection {* Logical consequence *}
+
+text {*
+  For every valuation, if all elements of @{text H} are true then so
+  is @{text p}.
+*}
+
+constdefs
+  sat :: "['a pl set, 'a pl] => bool"   (infixl "|=" 50)
+    "H |= p  ==  (\<forall>tt. (\<forall>q\<in>H. tt[[q]]) --> tt[[p]])"
+
+
+subsection {* Proof theory of propositional logic *}
+
+lemma thms_mono: "G<=H ==> thms(G) <= thms(H)"
+apply (unfold thms.defs )
+apply (rule lfp_mono)
+apply (assumption | rule basic_monos)+
+done
+
+lemma thms_I: "H |- p->p"
+  -- {*Called @{text I} for Identity Combinator, not for Introduction. *}
+by (best intro: thms.K thms.S thms.MP)
+
+
+subsubsection {* Weakening, left and right *}
+
+lemma weaken_left: "[| G \<subseteq> H;  G|-p |] ==> H|-p"
+  -- {* Order of premises is convenient with @{text THEN} *}
+  by (erule thms_mono [THEN subsetD])
+
+lemmas weaken_left_insert = subset_insertI [THEN weaken_left]
+
+lemmas weaken_left_Un1  = Un_upper1 [THEN weaken_left]
+lemmas weaken_left_Un2  = Un_upper2 [THEN weaken_left]
+
+lemma weaken_right: "H |- q ==> H |- p->q"
+by (fast intro: thms.K thms.MP)
+
+
+subsubsection {* The deduction theorem *}
+
+theorem deduction: "insert p H |- q  ==>  H |- p->q"
+apply (erule thms.induct)
+apply (fast intro: thms_I thms.H thms.K thms.S thms.DN 
+                   thms.S [THEN thms.MP, THEN thms.MP] weaken_right)+
+done
+
+
+subsubsection {* The cut rule *}
+
+lemmas cut = deduction [THEN thms.MP]
+
+lemmas thms_falseE = weaken_right [THEN thms.DN [THEN thms.MP]]
+
+lemmas thms_notE = thms.MP [THEN thms_falseE, standard]
+
+
+subsubsection {* Soundness of the rules wrt truth-table semantics *}
+
+theorem soundness: "H |- p ==> H |= p"
+apply (unfold sat_def)
+apply (erule thms.induct, auto) 
+done
+
+subsection {* Completeness *}
+
+subsubsection {* Towards the completeness proof *}
+
+lemma false_imp: "H |- p->false ==> H |- p->q"
+apply (rule deduction)
+apply (erule weaken_left_insert [THEN thms_notE])
+apply blast
+done
+
+lemma imp_false:
+    "[| H |- p;  H |- q->false |] ==> H |- (p->q)->false"
+apply (rule deduction)
+apply (blast intro: weaken_left_insert thms.MP thms.H) 
+done
+
+lemma hyps_thms_if: "hyps p tt |- (if tt[[p]] then p else p->false)"
+  -- {* Typical example of strengthening the induction statement. *}
+apply simp 
+apply (induct_tac "p")
+apply (simp_all add: thms_I thms.H)
+apply (blast intro: weaken_left_Un1 weaken_left_Un2 weaken_right
+                    imp_false false_imp)
+done
+
+lemma sat_thms_p: "{} |= p ==> hyps p tt |- p"
+  -- {* Key lemma for completeness; yields a set of assumptions 
+        satisfying @{text p} *}
+apply (unfold sat_def) 
+apply (drule spec, erule mp [THEN if_P, THEN subst], 
+       rule_tac [2] hyps_thms_if, simp)
+done
+
+text {*
+  For proving certain theorems in our new propositional logic.
+*}
+
+declare deduction [intro!]
+declare thms.H [THEN thms.MP, intro]
+
+text {*
+  The excluded middle in the form of an elimination rule.
+*}
+
+lemma thms_excluded_middle: "H |- (p->q) -> ((p->false)->q) -> q"
+apply (rule deduction [THEN deduction])
+apply (rule thms.DN [THEN thms.MP], best) 
+done
+
+lemma thms_excluded_middle_rule:
+    "[| insert p H |- q;  insert (p->false) H |- q |] ==> H |- q"
+  -- {* Hard to prove directly because it requires cuts *}
+by (rule thms_excluded_middle [THEN thms.MP, THEN thms.MP], auto) 
+
+
+subsection{* Completeness -- lemmas for reducing the set of assumptions*}
+
+text {*
+  For the case @{prop "hyps p t - insert #v Y |- p"} we also have @{prop
+  "hyps p t - {#v} \<subseteq> hyps p (t-{v})"}.
+*}
+
+lemma hyps_Diff: "hyps p (t-{v}) <= insert (#v->false) ((hyps p t)-{#v})"
+by (induct_tac "p", auto) 
+
+text {*
+  For the case @{prop "hyps p t - insert (#v -> Fls) Y |- p"} we also have
+  @{prop "hyps p t-{#v->Fls} \<subseteq> hyps p (insert v t)"}.
+*}
+
+lemma hyps_insert: "hyps p (insert v t) <= insert (#v) (hyps p t-{#v->false})"
+by (induct_tac "p", auto)
+
+text {* Two lemmas for use with @{text weaken_left} *}
+
+lemma insert_Diff_same: "B-C <= insert a (B-insert a C)"
+by fast
+
+lemma insert_Diff_subset2: "insert a (B-{c}) - D <= insert a (B-insert c D)"
+by fast
+
+text {*
+  The set @{term "hyps p t"} is finite, and elements have the form
+  @{term "#v"} or @{term "#v->Fls"}.
+*}
+
+lemma hyps_finite: "finite(hyps p t)"
+by (induct_tac "p", auto)
+
+lemma hyps_subset: "hyps p t <= (UN v. {#v, #v->false})"
+by (induct_tac "p", auto)
+
+lemmas Diff_weaken_left = Diff_mono [OF _ subset_refl, THEN weaken_left]
+
+subsubsection {* Completeness theorem *}
+
+text {*
+  Induction on the finite set of assumptions @{term "hyps p t0"}.  We
+  may repeatedly subtract assumptions until none are left!
+*}
+
+lemma completeness_0_lemma:
+    "{} |= p ==> \<forall>t. hyps p t - hyps p t0 |- p" 
+apply (rule hyps_subset [THEN hyps_finite [THEN finite_subset_induct]])
+ apply (simp add: sat_thms_p, safe)
+(*Case hyps p t-insert(#v,Y) |- p *)
+ apply (rule thms_excluded_middle_rule)
+  apply (rule insert_Diff_same [THEN weaken_left])
+  apply (erule spec)
+ apply (rule insert_Diff_subset2 [THEN weaken_left])
+ apply (rule hyps_Diff [THEN Diff_weaken_left])
+ apply (erule spec)
+(*Case hyps p t-insert(#v -> false,Y) |- p *)
+apply (rule thms_excluded_middle_rule)
+ apply (rule_tac [2] insert_Diff_same [THEN weaken_left])
+ apply (erule_tac [2] spec)
+apply (rule insert_Diff_subset2 [THEN weaken_left])
+apply (rule hyps_insert [THEN Diff_weaken_left])
+apply (erule spec)
+done
+
+text{*The base case for completeness*}
+lemma completeness_0:  "{} |= p ==> {} |- p"
+apply (rule Diff_cancel [THEN subst])
+apply (erule completeness_0_lemma [THEN spec])
+done
+
+text{*A semantic analogue of the Deduction Theorem*}
+lemma sat_imp: "insert p H |= q ==> H |= p->q"
+by (unfold sat_def, auto)
+
+theorem completeness [rule_format]: "finite H ==> \<forall>p. H |= p --> H |- p"
+apply (erule finite_induct)
+apply (safe intro!: completeness_0)
+apply (drule sat_imp)
+apply (drule spec) 
+apply (blast intro: weaken_left_insert [THEN thms.MP])  
+done
+
+theorem syntax_iff_semantics: "finite H ==> (H |- p) = (H |= p)"
+by (fast elim!: soundness completeness)
 
 end
 
