src/HOL/Induct/LList.thy
@@ -1,13 +1,11 @@
-(*  Title:      HOL/LList.thy
+(*  Title:      HOL/Induct/LList.thy
     ID:         $Id$
     Author:     Lawrence C Paulson, Cambridge University Computer Laboratory
     Copyright   1994  University of Cambridge
 
-Definition of type 'a llist by a greatest fixed point
-
 Shares NIL, CONS, List_case with List.thy
 
-Still needs filter and flatten functions -- hard because they need
+Still needs flatten function -- hard because it need
 bounds on the amount of lookahead required.
 
 Could try (but would it work for the gfp analogue of term?)
@@ -23,49 +21,53 @@ Previous definition of llistD_Fun was explicit:
        (UN x. (split(%l1 l2.(LCons(x,l1),LCons(x,l2))))`r)"
 *)
 
-LList = Main + SList +
+header {*Definition of type 'a llist by a greatest fixed point*}
+
+theory LList = Main + SList:
 
 consts
 
-  llist      :: 'a item set => 'a item set
-  LListD     :: "('a item * 'a item)set => ('a item * 'a item)set"
+  llist  :: "'a item set => 'a item set"
+  LListD :: "('a item * 'a item)set => ('a item * 'a item)set"
 
 
 coinductive "llist(A)"
-  intrs
-    NIL_I  "NIL: llist(A)"
-    CONS_I "[| a: A;  M: llist(A) |] ==> CONS a M : llist(A)"
+  intros
+    NIL_I:  "NIL \<in> llist(A)"
+    CONS_I:         "[| a \<in> A;  M \<in> llist(A) |] ==> CONS a M \<in> llist(A)"
 
 coinductive "LListD(r)"
-  intrs
-    NIL_I  "(NIL, NIL) : LListD(r)"
-    CONS_I "[| (a,b): r;  (M,N) : LListD(r)   
-            |] ==> (CONS a M, CONS b N) : LListD(r)"
+  intros
+    NIL_I:  "(NIL, NIL) \<in> LListD(r)"
+    CONS_I:         "[| (a,b) \<in> r;  (M,N) \<in> LListD(r) |] 
+                     ==> (CONS a M, CONS b N) \<in> LListD(r)"
 
 
 typedef (LList)
-  'a llist = "llist(range Leaf) :: 'a item set" (llist.NIL_I)
+  'a llist = "llist(range Leaf) :: 'a item set"
+  by (blast intro: llist.NIL_I)
 
 constdefs
-  (*Now used exclusively for abbreviating the coinduction rule*)
-  list_Fun   :: ['a item set, 'a item set] => 'a item set
-     "list_Fun A X == {z. z = NIL | (? M a. z = CONS a M & a : A & M : X)}"
+  list_Fun   :: "['a item set, 'a item set] => 'a item set"
+    --{*Now used exclusively for abbreviating the coinduction rule*}
+     "list_Fun A X == {z. z = NIL | (\<exists>M a. z = CONS a M & a \<in> A & M \<in> X)}"
 
   LListD_Fun :: 
       "[('a item * 'a item)set, ('a item * 'a item)set] => 
        ('a item * 'a item)set"
     "LListD_Fun r X ==   
        {z. z = (NIL, NIL) |   
-           (? M N a b. z = (CONS a M, CONS b N) & (a, b) : r & (M, N) : X)}"
+           (\<exists>M N a b. z = (CONS a M, CONS b N) & (a, b) \<in> r & (M, N) \<in> X)}"
 
-  (*the abstract constructors*)
-  LNil       :: 'a llist
+  LNil :: "'a llist"
+     --{*abstract constructor*}
     "LNil == Abs_LList NIL"
 
-  LCons      :: ['a, 'a llist] => 'a llist
+  LCons :: "['a, 'a llist] => 'a llist"
+     --{*abstract constructor*}
     "LCons x xs == Abs_LList(CONS (Leaf x) (Rep_LList xs))"
 
-  llist_case :: ['b, ['a, 'a llist]=>'b, 'a llist] => 'b
+  llist_case :: "['b, ['a, 'a llist]=>'b, 'a llist] => 'b"
     "llist_case c d l == 
        List_case c (%x y. d (inv Leaf x) (Abs_LList y)) (Rep_LList l)"
 
@@ -77,7 +79,7 @@ constdefs
              k"
 
   LList_corec     :: "['a, 'a => ('b item * 'a) option] => 'b item"
-    "LList_corec a f == UN k. LList_corec_fun k f a"
+    "LList_corec a f == \<Union>k. LList_corec_fun k f a"
 
   llist_corec     :: "['a, 'a => ('b * 'a) option] => 'b llist"
     "llist_corec a f == 
@@ -93,41 +95,810 @@ constdefs
 
 
 
-(*The case syntax for type 'a llist*)
+text{*The case syntax for type 'a llist*}
 translations
   "case p of LNil => a | LCons x l => b" == "llist_case a (%x l. b) p"
 
 
-(** Sample function definitions.  Item-based ones start with L ***)
+subsubsection{* Sample function definitions.  Item-based ones start with L *}
 
 constdefs
-  Lmap       :: ('a item => 'b item) => ('a item => 'b item)
+  Lmap       :: "('a item => 'b item) => ('a item => 'b item)"
     "Lmap f M == LList_corec M (List_case None (%x M'. Some((f(x), M'))))"
 
-  lmap       :: ('a=>'b) => ('a llist => 'b llist)
+  lmap       :: "('a=>'b) => ('a llist => 'b llist)"
     "lmap f l == llist_corec l (%z. case z of LNil => None 
                                            | LCons y z => Some(f(y), z))"
 
-  iterates   :: ['a => 'a, 'a] => 'a llist
+  iterates   :: "['a => 'a, 'a] => 'a llist"
     "iterates f a == llist_corec a (%x. Some((x, f(x))))"     
 
-  Lconst     :: 'a item => 'a item
-    "Lconst(M) == lfp(%N. CONS M N)"     
+  Lconst     :: "'a item => 'a item"
+    "Lconst(M) == lfp(%N. CONS M N)"
 
-(*Append generates its result by applying f, where
-    f((NIL,NIL))          = None
-    f((NIL, CONS N1 N2))  = Some((N1, (NIL,N2))
-    f((CONS M1 M2, N))    = Some((M1, (M2,N))
-*)
-
-  Lappend    :: ['a item, 'a item] => 'a item
+  Lappend    :: "['a item, 'a item] => 'a item"
    "Lappend M N == LList_corec (M,N)                                         
      (split(List_case (List_case None (%N1 N2. Some((N1, (NIL,N2))))) 
                       (%M1 M2 N. Some((M1, (M2,N))))))"
 
-  lappend    :: ['a llist, 'a llist] => 'a llist
+  lappend    :: "['a llist, 'a llist] => 'a llist"
     "lappend l n == llist_corec (l,n)                                         
        (split(llist_case (llist_case None (%n1 n2. Some((n1, (LNil,n2))))) 
                          (%l1 l2 n. Some((l1, (l2,n))))))"
+
+
+text{*Append generates its result by applying f, where
+    f((NIL,NIL))          = None
+    f((NIL, CONS N1 N2))  = Some((N1, (NIL,N2))
+    f((CONS M1 M2, N))    = Some((M1, (M2,N))
+*}
+
+text{*
+SHOULD LListD_Fun_CONS_I, etc., be equations (for rewriting)?
+*}
+
+lemmas UN1_I = UNIV_I [THEN UN_I, standard]
+
+subsubsection{* Simplification *}
+
+declare option.split [split]
+
+text{*This justifies using llist in other recursive type definitions*}
+lemma llist_mono: "A<=B ==> llist(A) <= llist(B)"
+apply (unfold llist.defs )
+apply (rule gfp_mono)
+apply (assumption | rule basic_monos)+
+done
+
+
+lemma llist_unfold: "llist(A) = usum {Numb(0)} (uprod A (llist A))"
+  by (fast intro!: llist.intros [unfolded NIL_def CONS_def]
+           elim: llist.cases [unfolded NIL_def CONS_def])
+
+
+subsection{* Type checking by coinduction, using list_Fun 
+     THE COINDUCTIVE DEFINITION PACKAGE COULD DO THIS!
+*}
+
+lemma llist_coinduct: 
+    "[| M \<in> X;  X <= list_Fun A (X Un llist(A)) |] ==>  M \<in> llist(A)"
+apply (unfold list_Fun_def)
+apply (erule llist.coinduct)
+apply (erule subsetD [THEN CollectD], assumption)
+done
+
+lemma list_Fun_NIL_I [iff]: "NIL \<in> list_Fun A X"
+by (unfold list_Fun_def NIL_def, fast)
+
+lemma list_Fun_CONS_I [intro!,simp]: 
+    "[| M \<in> A;  N \<in> X |] ==> CONS M N \<in> list_Fun A X"
+apply (unfold list_Fun_def CONS_def, fast)
+done
+
+
+text{*Utilise the "strong" part, i.e. gfp(f)*}
+lemma list_Fun_llist_I: "M \<in> llist(A) ==> M \<in> list_Fun A (X Un llist(A))"
+apply (unfold llist.defs list_Fun_def)
+apply (rule gfp_fun_UnI2) 
+apply (rule monoI, blast) 
+apply assumption
+done
+
+subsection{* LList_corec satisfies the desired recurion equation *}
+
+text{*A continuity result?*}
+lemma CONS_UN1: "CONS M (\<Union>x. f(x)) = (\<Union>x. CONS M (f x))"
+apply (unfold CONS_def)
+apply (simp add: In1_UN1 Scons_UN1_y)
+done
+
+lemma CONS_mono: "[| M<=M';  N<=N' |] ==> CONS M N <= CONS M' N'"
+apply (unfold CONS_def)
+apply (assumption | rule In1_mono Scons_mono)+
+done
+
+declare LList_corec_fun_def [THEN def_nat_rec_0, simp]
+        LList_corec_fun_def [THEN def_nat_rec_Suc, simp]
+
+subsubsection{* The directions of the equality are proved separately *}
+
+lemma LList_corec_subset1: 
+    "LList_corec a f <=  
+     (case f a of None => NIL | Some(z,w) => CONS z (LList_corec w f))"
+apply (unfold LList_corec_def)
+apply (rule UN_least)
+apply (case_tac "k")
+apply (simp_all (no_asm_simp))
+apply (rule allI impI subset_refl [THEN CONS_mono] UNIV_I [THEN UN_upper])+
+done
+
+lemma LList_corec_subset2: 
+    "(case f a of None => NIL | Some(z,w) => CONS z (LList_corec w f)) <=  
+     LList_corec a f"
+apply (unfold LList_corec_def)
+apply (simp add: CONS_UN1, safe) 
+apply (rule_tac a="Suc(?k)" in UN_I, simp, simp)+ 
+done
+
+text{*the recursion equation for LList_corec -- NOT SUITABLE FOR REWRITING!*}
+lemma LList_corec:
+     "LList_corec a f =   
+      (case f a of None => NIL | Some(z,w) => CONS z (LList_corec w f))"
+by (rule equalityI LList_corec_subset1 LList_corec_subset2)+
+
+text{*definitional version of same*}
+lemma def_LList_corec: 
+     "[| !!x. h(x) == LList_corec x f |]      
+      ==> h(a) = (case f a of None => NIL | Some(z,w) => CONS z (h w))"
+by (simp add: LList_corec)
+
+text{*A typical use of co-induction to show membership in the gfp. 
+  Bisimulation is  range(%x. LList_corec x f) *}
+lemma LList_corec_type: "LList_corec a f \<in> llist UNIV"
+apply (rule_tac X = "range (%x. LList_corec x ?g) " in llist_coinduct)
+apply (rule rangeI, safe)
+apply (subst LList_corec, simp)
+done
+
+
+subsection{* llist equality as a gfp; the bisimulation principle *}
+
+text{*This theorem is actually used, unlike the many similar ones in ZF*}
+lemma LListD_unfold: "LListD r = dsum (diag {Numb 0}) (dprod r (LListD r))"
+  by (fast intro!: LListD.intros [unfolded NIL_def CONS_def]
+           elim: LListD.cases [unfolded NIL_def CONS_def])
+
+lemma LListD_implies_ntrunc_equality [rule_format]:
+     "\<forall>M N. (M,N) \<in> LListD(diag A) --> ntrunc k M = ntrunc k N"
+apply (induct_tac "k" rule: nat_less_induct)
+apply (safe del: equalityI)
+apply (erule LListD.cases)
+apply (safe del: equalityI)
+apply (case_tac "n", simp)
+apply (rename_tac "n'")
+apply (case_tac "n'")
+apply (simp_all add: CONS_def less_Suc_eq)
+done
+
+text{*The domain of the LListD relation*}
+lemma Domain_LListD: 
+    "Domain (LListD(diag A)) <= llist(A)"
+apply (unfold llist.defs NIL_def CONS_def)
+apply (rule gfp_upperbound)
+txt{*avoids unfolding LListD on the rhs*}
+apply (rule_tac P = "%x. Domain x <= ?B" in LListD_unfold [THEN ssubst], simp)
+apply blast 
+done
+
+text{*This inclusion justifies the use of coinduction to show M=N*}
+lemma LListD_subset_diag: "LListD(diag A) <= diag(llist(A))"
+apply (rule subsetI)
+apply (rule_tac p = "x" in PairE, safe)
+apply (rule diag_eqI)
+apply (rule LListD_implies_ntrunc_equality [THEN ntrunc_equality], assumption)
+apply (erule DomainI [THEN Domain_LListD [THEN subsetD]])
+done
+
+
+subsubsection{* Coinduction, using LListD_Fun
+    THE COINDUCTIVE DEFINITION PACKAGE COULD DO THIS!
+ *}
+
+lemma LListD_Fun_mono: "A<=B ==> LListD_Fun r A <= LListD_Fun r B"
+apply (unfold LListD_Fun_def)
+apply (assumption | rule basic_monos)+
+done
+
+lemma LListD_coinduct: 
+    "[| M \<in> X;  X <= LListD_Fun r (X Un LListD(r)) |] ==>  M \<in> LListD(r)"
+apply (unfold LListD_Fun_def)
+apply (erule LListD.coinduct)
+apply (erule subsetD [THEN CollectD], assumption)
+done
+
+lemma LListD_Fun_NIL_I: "(NIL,NIL) \<in> LListD_Fun r s"
+by (unfold LListD_Fun_def NIL_def, fast)
+
+lemma LListD_Fun_CONS_I: 
+     "[| x\<in>A;  (M,N):s |] ==> (CONS x M, CONS x N) \<in> LListD_Fun (diag A) s"
+apply (unfold LListD_Fun_def CONS_def, blast)
+done
+
+text{*Utilise the "strong" part, i.e. gfp(f)*}
+lemma LListD_Fun_LListD_I:
+     "M \<in> LListD(r) ==> M \<in> LListD_Fun r (X Un LListD(r))"
+apply (unfold LListD.defs LListD_Fun_def)
+apply (rule gfp_fun_UnI2) 
+apply (rule monoI, blast) 
+apply assumption
+done
+
+
+text{*This converse inclusion helps to strengthen LList_equalityI*}
+lemma diag_subset_LListD: "diag(llist(A)) <= LListD(diag A)"
+apply (rule subsetI)
+apply (erule LListD_coinduct)
+apply (rule subsetI)
+apply (erule diagE)
+apply (erule ssubst)
+apply (erule llist.cases)
+apply (simp_all add: diagI LListD_Fun_NIL_I LListD_Fun_CONS_I)
+done
+
+lemma LListD_eq_diag: "LListD(diag A) = diag(llist(A))"
+apply (rule equalityI LListD_subset_diag diag_subset_LListD)+
+done
+
+lemma LListD_Fun_diag_I: "M \<in> llist(A) ==> (M,M) \<in> LListD_Fun (diag A) (X Un diag(llist(A)))"
+apply (rule LListD_eq_diag [THEN subst])
+apply (rule LListD_Fun_LListD_I)
+apply (simp add: LListD_eq_diag diagI)
+done
+
+
+subsubsection{* To show two LLists are equal, exhibit a bisimulation! 
+      [also admits true equality]
+   Replace "A" by some particular set, like {x.True}??? *}
+lemma LList_equalityI:
+     "[| (M,N) \<in> r;  r <= LListD_Fun (diag A) (r Un diag(llist(A))) |] 
+      ==>  M=N"
+apply (rule LListD_subset_diag [THEN subsetD, THEN diagE])
+apply (erule LListD_coinduct)
+apply (simp add: LListD_eq_diag, safe)
+done
+
+
+subsection{* Finality of llist(A): Uniqueness of functions defined by corecursion *}
+
+text{*We must remove Pair_eq because it may turn an instance of reflexivity
+  (h1 b, h2 b) = (h1 ?x17, h2 ?x17) into a conjunction! 
+  (or strengthen the Solver?) 
+*}
+declare Pair_eq [simp del]
+
+text{*abstract proof using a bisimulation*}
+lemma LList_corec_unique:
+ "[| !!x. h1(x) = (case f x of None => NIL | Some(z,w) => CONS z (h1 w));   
+     !!x. h2(x) = (case f x of None => NIL | Some(z,w) => CONS z (h2 w)) |] 
+  ==> h1=h2"
+apply (rule ext)
+txt{*next step avoids an unknown (and flexflex pair) in simplification*}
+apply (rule_tac A = "UNIV" and r = "range(%u. (h1 u, h2 u))" 
+       in LList_equalityI)
+apply (rule rangeI, safe)
+apply (simp add: LListD_Fun_NIL_I UNIV_I [THEN LListD_Fun_CONS_I])
+done
+
+lemma equals_LList_corec:
+ "[| !!x. h(x) = (case f x of None => NIL | Some(z,w) => CONS z (h w)) |]  
+  ==> h = (%x. LList_corec x f)"
+by (simp add: LList_corec_unique LList_corec) 
+
+
+subsubsection{*Obsolete proof of @{text LList_corec_unique}: 
+               complete induction, not coinduction *}
+
+lemma ntrunc_one_CONS [simp]: "ntrunc (Suc 0) (CONS M N) = {}"
+by (simp add: CONS_def ntrunc_one_In1)
+
+lemma ntrunc_CONS [simp]: 
+    "ntrunc (Suc(Suc(k))) (CONS M N) = CONS (ntrunc k M) (ntrunc k N)"
+by (simp add: CONS_def)
+
+
+lemma
+ assumes prem1:
+          "!!x. h1 x = (case f x of None => NIL | Some(z,w) => CONS z (h1 w))"
+     and prem2:
+          "!!x. h2 x = (case f x of None => NIL | Some(z,w) => CONS z (h2 w))"
+ shows "h1=h2"
+apply (rule ntrunc_equality [THEN ext])
+apply (rule_tac x = "x" in spec)
+apply (induct_tac "k" rule: nat_less_induct)
+apply (rename_tac "n")
+apply (rule allI)
+apply (subst prem1)
+apply (subst prem2, simp)
+apply (intro strip) 
+apply (case_tac "n") 
+apply (rename_tac [2] "m")
+apply (case_tac [2] "m")
+apply simp_all
+done
+
+
+subsection{*Lconst: defined directly by lfp *}
+
+text{*But it could be defined by corecursion.*}
+
+lemma Lconst_fun_mono: "mono(CONS(M))"
+apply (rule monoI subset_refl CONS_mono)+
+apply assumption 
+done
+
+text{* Lconst(M) = CONS M (Lconst M) *}
+lemmas Lconst = Lconst_fun_mono [THEN Lconst_def [THEN def_lfp_unfold]]
+
+text{*A typical use of co-induction to show membership in the gfp.
+  The containing set is simply the singleton {Lconst(M)}. *}
+lemma Lconst_type: "M\<in>A ==> Lconst(M): llist(A)"
+apply (rule singletonI [THEN llist_coinduct], safe)
+apply (rule_tac P = "%u. u \<in> ?A" in Lconst [THEN ssubst])
+apply (assumption | rule list_Fun_CONS_I singletonI UnI1)+
+done
+
+lemma Lconst_eq_LList_corec: "Lconst(M) = LList_corec M (%x. Some(x,x))"
+apply (rule equals_LList_corec [THEN fun_cong], simp)
+apply (rule Lconst)
+done
+
+text{*Thus we could have used gfp in the definition of Lconst*}
+lemma gfp_Lconst_eq_LList_corec: "gfp(%N. CONS M N) = LList_corec M (%x. Some(x,x))"
+apply (rule equals_LList_corec [THEN fun_cong], simp)
+apply (rule Lconst_fun_mono [THEN gfp_unfold])
+done
+
+
+subsection{* Isomorphisms *}
+
+lemma inj_Rep_LList: "inj Rep_LList"
+apply (rule inj_inverseI)
+apply (rule Rep_LList_inverse)
+done
+
+
+lemma LListI: "x \<in> llist (range Leaf) ==> x \<in> LList"
+by (unfold LList_def, simp)
+
+lemma LListD: "x \<in> LList ==> x \<in> llist (range Leaf)"
+by (unfold LList_def, simp)
+
+
+subsubsection{* Distinctness of constructors *}
+
+lemma LCons_not_LNil [iff]: "~ LCons x xs = LNil"
+apply (unfold LNil_def LCons_def)
+apply (subst Abs_LList_inject)
+apply (rule llist.intros CONS_not_NIL rangeI LListI Rep_LList [THEN LListD])+
+done
+
+lemmas LNil_not_LCons [iff] = LCons_not_LNil [THEN not_sym, standard]
+
+
+subsubsection{* llist constructors *}
+
+lemma Rep_LList_LNil: "Rep_LList LNil = NIL"
+apply (unfold LNil_def)
+apply (rule llist.NIL_I [THEN LListI, THEN Abs_LList_inverse])
+done
+
+lemma Rep_LList_LCons: "Rep_LList(LCons x l) = CONS (Leaf x) (Rep_LList l)"
+apply (unfold LCons_def)
+apply (rule llist.CONS_I [THEN LListI, THEN Abs_LList_inverse] 
+            rangeI Rep_LList [THEN LListD])+
+done
+
+subsubsection{* Injectiveness of CONS and LCons *}
+
+lemma CONS_CONS_eq2: "(CONS M N=CONS M' N') = (M=M' & N=N')"
+apply (unfold CONS_def)
+apply (fast elim!: Scons_inject)
+done
+
+lemmas CONS_inject = CONS_CONS_eq [THEN iffD1, THEN conjE, standard]
+
+
+text{*For reasoning about abstract llist constructors*}
+
+declare Rep_LList [THEN LListD, intro] LListI [intro]
+declare llist.intros [intro]
+
+lemma LCons_LCons_eq [iff]: "(LCons x xs=LCons y ys) = (x=y & xs=ys)"
+apply (unfold LCons_def)
+apply (subst Abs_LList_inject)
+apply (auto simp add: Rep_LList_inject)
+done
+
+lemma LList_fun_equalityI: "CONS M N \<in> llist(A) ==> M \<in> A & N \<in> llist(A)"
+apply (erule llist.cases)
+apply (erule CONS_neq_NIL, fast)
+done
+
+
+subsection{* Reasoning about llist(A) *}
+
+text{*A special case of list_equality for functions over lazy lists*}
+lemma LList_fun_equalityI:
+ "[| M \<in> llist(A); g(NIL): llist(A);                              
+     f(NIL)=g(NIL);                                              
+     !!x l. [| x\<in>A;  l \<in> llist(A) |] ==>                          
+            (f(CONS x l),g(CONS x l)) \<in>                          
+                LListD_Fun (diag A) ((%u.(f(u),g(u)))`llist(A) Un   
+                                    diag(llist(A)))              
+  |] ==> f(M) = g(M)"
+apply (rule LList_equalityI)
+apply (erule imageI)
+apply (rule image_subsetI)
+apply (erule_tac aa=x in llist.cases)
+apply (erule ssubst, erule ssubst, erule LListD_Fun_diag_I, blast) 
+done
+
+
+subsection{* The functional "Lmap" *}
+
+lemma Lmap_NIL [simp]: "Lmap f NIL = NIL"
+by (rule Lmap_def [THEN def_LList_corec, THEN trans], simp)
+
+lemma Lmap_CONS [simp]: "Lmap f (CONS M N) = CONS (f M) (Lmap f N)"
+by (rule Lmap_def [THEN def_LList_corec, THEN trans], simp)
+
+
+
+text{*Another type-checking proof by coinduction*}
+lemma Lmap_type:
+     "[| M \<in> llist(A);  !!x. x\<in>A ==> f(x):B |] ==> Lmap f M \<in> llist(B)"
+apply (erule imageI [THEN llist_coinduct], safe)
+apply (erule llist.cases, simp_all)
+done
+
+text{*This type checking rule synthesises a sufficiently large set for f*}
+lemma Lmap_type2: "M \<in> llist(A) ==> Lmap f M \<in> llist(f`A)"
+apply (erule Lmap_type)
+apply (erule imageI)
+done
+
+subsubsection{* Two easy results about Lmap *}
+
+lemma Lmap_compose: "M \<in> llist(A) ==> Lmap (f o g) M = Lmap f (Lmap g M)"
+apply (unfold o_def)
+apply (drule imageI)
+apply (erule LList_equalityI, safe)
+apply (erule llist.cases, simp_all)
+apply (rule LListD_Fun_NIL_I imageI UnI1 rangeI [THEN LListD_Fun_CONS_I])+
+apply assumption  
+done
+
+lemma Lmap_ident: "M \<in> llist(A) ==> Lmap (%x. x) M = M"
+apply (drule imageI)
+apply (erule LList_equalityI, safe)
+apply (erule llist.cases, simp_all)
+apply (rule LListD_Fun_NIL_I imageI UnI1 rangeI [THEN LListD_Fun_CONS_I])+
+apply assumption 
+done
+
+
+subsection{* Lappend -- its two arguments cause some complications! *}
+
+lemma Lappend_NIL_NIL [simp]: "Lappend NIL NIL = NIL"
+apply (unfold Lappend_def)
+apply (rule LList_corec [THEN trans], simp)
+done
+
+lemma Lappend_NIL_CONS [simp]: 
+    "Lappend NIL (CONS N N') = CONS N (Lappend NIL N')"
+apply (unfold Lappend_def)
+apply (rule LList_corec [THEN trans], simp)
+done
+
+lemma Lappend_CONS [simp]: 
+    "Lappend (CONS M M') N = CONS M (Lappend M' N)"
+apply (unfold Lappend_def)
+apply (rule LList_corec [THEN trans], simp)
+done
+
+declare llist.intros [simp] LListD_Fun_CONS_I [simp] 
+        range_eqI [simp] image_eqI [simp]
+
+
+lemma Lappend_NIL [simp]: "M \<in> llist(A) ==> Lappend NIL M = M"
+by (erule LList_fun_equalityI, simp_all)
+
+lemma Lappend_NIL2: "M \<in> llist(A) ==> Lappend M NIL = M"
+by (erule LList_fun_equalityI, simp_all)
+
+
+subsubsection{* Alternative type-checking proofs for Lappend *}
+
+text{*weak co-induction: bisimulation and case analysis on both variables*}
+lemma Lappend_type: "[| M \<in> llist(A); N \<in> llist(A) |] ==> Lappend M N \<in> llist(A)"
+apply (rule_tac X = "\<Union>u\<in>llist (A) . \<Union>v \<in> llist (A) . {Lappend u v}" in llist_coinduct)
+apply fast
+apply safe
+apply (erule_tac aa = "u" in llist.cases)
+apply (erule_tac aa = "v" in llist.cases, simp_all)
+apply blast
+done
+
+text{*strong co-induction: bisimulation and case analysis on one variable*}
+lemma Lappend_type: "[| M \<in> llist(A); N \<in> llist(A) |] ==> Lappend M N \<in> llist(A)"
+apply (rule_tac X = " (%u. Lappend u N) `llist (A) " in llist_coinduct)
+apply (erule imageI)
+apply (rule image_subsetI)
+apply (erule_tac aa = "x" in llist.cases)
+apply (simp add: list_Fun_llist_I, simp)
+done
+
+subsection{* Lazy lists as the type 'a llist -- strongly typed versions of above *}
+
+subsubsection{* llist_case: case analysis for 'a llist *}
+
+declare LListI [THEN Abs_LList_inverse, simp]
+declare Rep_LList_inverse [simp]
+declare Rep_LList [THEN LListD, simp]
+declare rangeI [simp] inj_Leaf [simp] 
+
+lemma llist_case_LNil [simp]: "llist_case c d LNil = c"
+by (unfold llist_case_def LNil_def, simp)
+
+lemma llist_case_LCons [simp]: 
+    "llist_case c d (LCons M N) = d M N"
+apply (unfold llist_case_def LCons_def, simp)
+done
+
+text{*Elimination is case analysis, not induction.*}
+lemma llistE: "[| l=LNil ==> P;  !!x l'. l=LCons x l' ==> P |] ==> P"
+apply (rule Rep_LList [THEN LListD, THEN llist.cases])
+ apply (simp add: Rep_LList_LNil [symmetric] Rep_LList_inject)
+ apply blast 
+apply (erule LListI [THEN Rep_LList_cases], clarify)
+apply (simp add: Rep_LList_LCons [symmetric] Rep_LList_inject, blast) 
+done
+
+subsubsection{* llist_corec: corecursion for 'a llist *}
+
+text{*Lemma for the proof of llist_corec*}
+lemma LList_corec_type2:
+     "LList_corec a  
+           (%z. case f z of None => None | Some(v,w) => Some(Leaf(v),w)) 
+       \<in> llist(range Leaf)"
+apply (rule_tac X = "range (%x. LList_corec x ?g) " in llist_coinduct)
+apply (rule rangeI, safe)
+apply (subst LList_corec, force)
+done
+
+lemma llist_corec: 
+    "llist_corec a f =   
+     (case f a of None => LNil | Some(z,w) => LCons z (llist_corec w f))"
+apply (unfold llist_corec_def LNil_def LCons_def)
+apply (subst LList_corec)
+apply (case_tac "f a")
+apply (simp add: LList_corec_type2)
+apply (force simp add: LList_corec_type2)
+done
+
+text{*definitional version of same*}
+lemma def_llist_corec: 
+     "[| !!x. h(x) == llist_corec x f |] ==>      
+      h(a) = (case f a of None => LNil | Some(z,w) => LCons z (h w))"
+by (simp add: llist_corec)
+
+subsection{* Proofs about type 'a llist functions *}
+
+subsection{* Deriving llist_equalityI -- llist equality is a bisimulation *}
+
+lemma LListD_Fun_subset_Times_llist: 
+    "r <= (llist A) <*> (llist A) ==>  
+            LListD_Fun (diag A) r <= (llist A) <*> (llist A)"
+apply (unfold LListD_Fun_def)
+apply (subst llist_unfold)
+apply (simp add: NIL_def CONS_def, fast)
+done
+
+lemma subset_Times_llist:
+     "prod_fun Rep_LList Rep_LList ` r <=  
+     (llist(range Leaf)) <*> (llist(range Leaf))"
+by (blast intro: Rep_LList [THEN LListD])
+
+lemma prod_fun_lemma:
+     "r <= (llist(range Leaf)) <*> (llist(range Leaf)) 
+      ==> prod_fun (Rep_LList o Abs_LList) (Rep_LList o Abs_LList) ` r <= r"
+apply safe
+apply (erule subsetD [THEN SigmaE2], assumption)
+apply (simp add: LListI [THEN Abs_LList_inverse])
+done
+
+lemma prod_fun_range_eq_diag:
+     "prod_fun Rep_LList  Rep_LList ` range(%x. (x, x)) =  
+      diag(llist(range Leaf))"
+apply (rule equalityI, blast) 
+apply (fast elim: LListI [THEN Abs_LList_inverse, THEN subst])
+done
+
+text{*Used with lfilter*}
+lemma llistD_Fun_mono: 
+    "A<=B ==> llistD_Fun A <= llistD_Fun B"
+apply (unfold llistD_Fun_def prod_fun_def, auto)
+apply (rule image_eqI)
+ prefer 2 apply (blast intro: rev_subsetD [OF _ LListD_Fun_mono], force)
+done
+
+subsubsection{* To show two llists are equal, exhibit a bisimulation! 
+      [also admits true equality] *}
+lemma llist_equalityI: 
+    "[| (l1,l2) \<in> r;  r <= llistD_Fun(r Un range(%x.(x,x))) |] ==> l1=l2"
+apply (unfold llistD_Fun_def)
+apply (rule Rep_LList_inject [THEN iffD1])
+apply (rule_tac r = "prod_fun Rep_LList Rep_LList `r" and A = "range (Leaf) " in LList_equalityI)
+apply (erule prod_fun_imageI)
+apply (erule image_mono [THEN subset_trans])
+apply (rule image_compose [THEN subst])
+apply (rule prod_fun_compose [THEN subst])
+apply (subst image_Un)
+apply (subst prod_fun_range_eq_diag)
+apply (rule LListD_Fun_subset_Times_llist [THEN prod_fun_lemma])
+apply (rule subset_Times_llist [THEN Un_least])
+apply (rule diag_subset_Times)
+done
+
+subsubsection{* Rules to prove the 2nd premise of llist_equalityI *}
+lemma llistD_Fun_LNil_I [simp]: "(LNil,LNil) \<in> llistD_Fun(r)"
+apply (unfold llistD_Fun_def LNil_def)
+apply (rule LListD_Fun_NIL_I [THEN prod_fun_imageI])
+done
+
+lemma llistD_Fun_LCons_I [simp]: 
+    "(l1,l2):r ==> (LCons x l1, LCons x l2) \<in> llistD_Fun(r)"
+apply (unfold llistD_Fun_def LCons_def)
+apply (rule rangeI [THEN LListD_Fun_CONS_I, THEN prod_fun_imageI])
+apply (erule prod_fun_imageI)
+done
+
+text{*Utilise the "strong" part, i.e. gfp(f)*}
+lemma llistD_Fun_range_I: "(l,l) \<in> llistD_Fun(r Un range(%x.(x,x)))"
+apply (unfold llistD_Fun_def)
+apply (rule Rep_LList_inverse [THEN subst])
+apply (rule prod_fun_imageI)
+apply (subst image_Un)
+apply (subst prod_fun_range_eq_diag)
+apply (rule Rep_LList [THEN LListD, THEN LListD_Fun_diag_I])
+done
+
+text{*A special case of list_equality for functions over lazy lists*}
+lemma llist_fun_equalityI:
+     "[| f(LNil)=g(LNil);                                                 
+         !!x l. (f(LCons x l),g(LCons x l)) 
+                \<in> llistD_Fun(range(%u. (f(u),g(u))) Un range(%v. (v,v)))    
+      |] ==> f(l) = (g(l :: 'a llist) :: 'b llist)"
+apply (rule_tac r = "range (%u. (f (u),g (u))) " in llist_equalityI)
+apply (rule rangeI, clarify) 
+apply (rule_tac l = "u" in llistE)
+apply (simp_all add: llistD_Fun_range_I) 
+done
+
+
+subsection{* The functional "lmap" *}
+
+lemma lmap_LNil [simp]: "lmap f LNil = LNil"
+by (rule lmap_def [THEN def_llist_corec, THEN trans], simp)
+
+lemma lmap_LCons [simp]: "lmap f (LCons M N) = LCons (f M) (lmap f N)"
+by (rule lmap_def [THEN def_llist_corec, THEN trans], simp)
+
+
+subsubsection{* Two easy results about lmap *}
+
+lemma lmap_compose [simp]: "lmap (f o g) l = lmap f (lmap g l)"
+by (rule_tac l = "l" in llist_fun_equalityI, simp_all)
+
+lemma lmap_ident [simp]: "lmap (%x. x) l = l"
+by (rule_tac l = "l" in llist_fun_equalityI, simp_all)
+
+
+subsection{* iterates -- llist_fun_equalityI cannot be used! *}
+
+lemma iterates: "iterates f x = LCons x (iterates f (f x))"
+by (rule iterates_def [THEN def_llist_corec, THEN trans], simp)
+
+lemma lmap_iterates [simp]: "lmap f (iterates f x) = iterates f (f x)"
+apply (rule_tac r = "range (%u. (lmap f (iterates f u),iterates f (f u))) " in llist_equalityI)
+apply (rule rangeI, safe)
+apply (rule_tac x1 = "f (u) " in iterates [THEN ssubst])
+apply (rule_tac x1 = "u" in iterates [THEN ssubst], simp)
+done
+
+lemma iterates_lmap: "iterates f x = LCons x (lmap f (iterates f x))"
+apply (subst lmap_iterates)
+apply (rule iterates)
+done
+
+subsection{* A rather complex proof about iterates -- cf Andy Pitts *}
+
+subsubsection{* Two lemmas about natrec n x (%m.g), which is essentially (g^n)(x) *}
+
+lemma fun_power_lmap: "nat_rec (LCons b l) (%m. lmap(f)) n =       
+     LCons (nat_rec b (%m. f) n) (nat_rec l (%m. lmap(f)) n)"
+apply (induct_tac "n", simp_all)
+done
+
+lemma fun_power_Suc: "nat_rec (g x) (%m. g) n = nat_rec x (%m. g) (Suc n)"
+by (induct_tac "n", simp_all)
+
+lemmas Pair_cong = refl [THEN cong, THEN cong, of concl: Pair]
+
+
+text{*The bisimulation consists of {(lmap(f)^n (h(u)), lmap(f)^n (iterates(f,u)))}
+  for all u and all n::nat.*}
+lemma iterates_equality:
+     "(!!x. h(x) = LCons x (lmap f (h x))) ==> h = iterates(f)"
+apply (rule ext)
+apply (rule_tac 
+       r = "\<Union>u. range (%n. (nat_rec (h u) (%m y. lmap f y) n, 
+                             nat_rec (iterates f u) (%m y. lmap f y) n))" 
+       in llist_equalityI)
+apply (rule UN1_I range_eqI Pair_cong nat_rec_0 [symmetric])+
+apply clarify
+apply (subst iterates, atomize)
+apply (drule_tac x=u in spec) 
+apply (erule ssubst) 
+apply (subst fun_power_lmap)
+apply (subst fun_power_lmap)
+apply (rule llistD_Fun_LCons_I)
+apply (rule lmap_iterates [THEN subst])
+apply (subst fun_power_Suc)
+apply (subst fun_power_Suc, blast)
+done
+
+
+subsection{* lappend -- its two arguments cause some complications! *}
+
+lemma lappend_LNil_LNil [simp]: "lappend LNil LNil = LNil"
+apply (unfold lappend_def)
+apply (rule llist_corec [THEN trans], simp)
+done
+
+lemma lappend_LNil_LCons [simp]: 
+    "lappend LNil (LCons l l') = LCons l (lappend LNil l')"
+apply (unfold lappend_def)
+apply (rule llist_corec [THEN trans], simp)
+done
+
+lemma lappend_LCons [simp]: 
+    "lappend (LCons l l') N = LCons l (lappend l' N)"
+apply (unfold lappend_def)
+apply (rule llist_corec [THEN trans], simp)
+done
+
+lemma lappend_LNil [simp]: "lappend LNil l = l"
+by (rule_tac l = "l" in llist_fun_equalityI, simp_all)
+
+lemma lappend_LNil2 [simp]: "lappend l LNil = l"
+by (rule_tac l = "l" in llist_fun_equalityI, simp_all)
+
+
+text{*The infinite first argument blocks the second*}
+lemma lappend_iterates [simp]: "lappend (iterates f x) N = iterates f x"
+apply (rule_tac r = "range (%u. (lappend (iterates f u) N,iterates f u))" 
+       in llist_equalityI)
+apply (rule rangeI, safe)
+apply (subst iterates, simp)
+done
+
+subsubsection{* Two proofs that lmap distributes over lappend *}
+
+text{*Long proof requiring case analysis on both both arguments*}
+lemma lmap_lappend_distrib:
+     "lmap f (lappend l n) = lappend (lmap f l) (lmap f n)"
+apply (rule_tac r = "\<Union>n. range (%l. (lmap f (lappend l n),
+                                      lappend (lmap f l) (lmap f n)))" 
+       in llist_equalityI)
+apply (rule UN1_I)
+apply (rule rangeI, safe)
+apply (rule_tac l = "l" in llistE)
+apply (rule_tac l = "n" in llistE, simp_all)
+apply (blast intro: llistD_Fun_LCons_I) 
+done
+
+text{*Shorter proof of theorem above using llist_equalityI as strong coinduction*}
+lemma lmap_lappend_distrib:
+     "lmap f (lappend l n) = lappend (lmap f l) (lmap f n)"
+apply (rule_tac l = "l" in llist_fun_equalityI, simp)
+apply simp
+done
+
+text{*Without strong coinduction, three case analyses might be needed*}
+lemma lappend_assoc: "lappend (lappend l1 l2) l3 = lappend l1 (lappend l2 l3)"
+apply (rule_tac l = "l1" in llist_fun_equalityI, simp)
+apply simp
+done
 
 end
